UnitProJ/expressOS/August/INode.dfy
@@ -62,7 +62,6 @@ spine == [this] + next.spine && footprint == {this} + next.footprint
 && next.ValidLemma2())
 }
 
-
 constructor init(d:Data) 
 modifies this;
 ensures Valid();
@@ -170,15 +169,27 @@ else
 allV(myNode.next)
 }
 
+predicate seqV(mySeq: seq<INode>)
+requires goodSeqCond(mySeq);
+requires mySeq != [] ==> mySeq[0].Valid();
+
+reads mySeq, sumAllFtprint(mySeq);
+ensures seqV(mySeq);
+ensures goodSeqCond(mySeq);
+ensures forall nd :: nd in mySeq ==> nd.Valid(); 
+{
+mySeq == [] ||
+(seqV(mySeq[1..]))
+}
 
 
 predicate listCond(mySeq: seq<INode>)
 reads mySeq, (set nd | nd in mySeq);
 {
 null !in mySeq &&
-(forall nd :: nd in mySeq ==> nd in nd.footprint) &&
-(forall i :: 0 <= i < |mySeq|-1 ==> mySeq[i].next == mySeq[i+1]
-			&& mySeq[i] !in mySeq[i+1..])
+(forall i :: 0 <= i < |mySeq|-1 ==> mySeq[i].next == mySeq[i+1])
+&& (mySeq != [] ==> mySeq[|mySeq|-1].next == null)
+&& (forall i, j :: 0 <= i < j < |mySeq| ==> mySeq[i] !in mySeq[j].footprint)
 }
 
 predicate goodSeqCond(mySeq: seq<INode>)
@@ -195,23 +206,22 @@ listCond(mySeq) &&
 (forall nd :: nd in mySeq ==> nd.Valid())
 }
 
-//===============================================
-/*
 
-//The nodes on the l.h.s of index are all good,
-//while all the nodes on the r.h.s of index are Valid.
+//===============================================
+
 
 ghost method updateCurIndex(mySeq:seq<INode>, index:int)
 requires 0 <= index <= |mySeq| - 2;
 requires listCond(mySeq);
-
-requires mySeq[index+1].Valid();
-requires mySeq[index] !in (mySeq[index+1..]);
+requires index > 0 ==> goodSeqCond(mySeq[0..index]);
+requires validSeqCond(mySeq[index+1..]);
+	
 //requires mySeq[index] !in (mySeq[index+1].footprint);
 
 modifies mySeq;
 ensures fresh((set nd | nd in mySeq) - old(set nd | nd in mySeq));
 ensures listCond(mySeq);
+
 ensures mySeq[index].Valid(); 
 {
 mySeq[index].tailContents := [mySeq[index+1].data] + mySeq[index+1].tailContents;
@@ -223,7 +233,7 @@ mySeq[index].spine := [mySeq[index]] + mySeq[index+1].spine;
 }
 
 
-
+/*
 ghost method updateSeq(mySeq:seq<INode>)
 
 requires mySeq != [];
@@ -280,8 +290,9 @@ assert mySeq[|mySeq|-1].next == null;
 */
 }
 
+assert seqV(mySeq);
+
 }
 */
 
 }
-
